proof/SimMemInjNew.v
@@ -1,0 +1,529 @@
+Require Import CoqlibC.
+Require Import Memory.
+Require Import Values.
+Require Import Maps.
+Require Import Events.
+Require Import Globalenvs.
+Require Import AST.
+
+Require Import IntegersC LinkingC.
+Require Import SimDef SimSymb Skeleton Mod ModSem.
+Require Import SimMem.
+
+Set Implicit Arguments.
+
+(* Copied from CRELLVM *)
+Inductive frozen (f_old f_new: meminj) (bound_src bound_tgt: block): Prop :=
+| frozen_intro
+    (NEW_IMPLIES_OUTSIDE:
+       forall b_src b_tgt delta
+              (NEW: f_old b_src = None /\ f_new b_src = Some(b_tgt, delta)),
+         <<OUTSIDE_SRC: (bound_src <= b_src)%positive>> /\ <<OUTSIDE_TGT: (bound_tgt <= b_tgt)%positive>>)
+.
+
+Remark inject_separated_frozen
+       f_old f_new m_src m_tgt
+  :
+    Events.inject_separated f_old f_new m_src m_tgt <->
+    frozen f_old f_new m_src.(Mem.nextblock) m_tgt.(Mem.nextblock)
+.
+Proof.
+  unfold Events.inject_separated in *.
+  unfold Mem.valid_block in *.
+  split; i.
+  - econs; eauto.
+    i. des.
+    hexploit H; eauto. i; des.
+    splits; xomega.
+  - inv H.
+    exploit NEW_IMPLIES_OUTSIDE; eauto.
+    i; des.
+    split; xomega.
+Qed.
+
+Lemma frozen_preserves_src
+      f_old f_new
+      (INJECT: inject_incr f_old f_new)
+      bound_src bound_tgt
+      (FROZEN: frozen f_old f_new bound_src bound_tgt)
+      b_src
+      (INSIDE: (b_src < bound_src)%positive)
+  :
+    <<PRESERVED: f_old b_src = f_new b_src>>
+.
+Proof.
+  inv FROZEN.
+  destruct (f_old b_src) eqn:T0; ss;
+    destruct (f_new b_src) eqn:T1; ss.
+  - destruct p, p0; ss.
+    exploit INJECT; eauto; []; i; des.
+    clarify.
+  - destruct p; ss.
+    exploit INJECT; eauto; []; i; des.
+    clarify.
+  - destruct p; ss.
+    exploit NEW_IMPLIES_OUTSIDE; eauto; []; i; des.
+    exfalso.
+    xomega.
+Qed.
+
+Lemma frozen_preserves_tgt
+      f_old f_new
+      (INJECT: inject_incr f_old f_new)
+      bound_src bound_tgt
+      (FROZEN: frozen f_old f_new bound_src bound_tgt)
+      b_tgt
+      (INSIDE: (b_tgt < bound_tgt)%positive)
+  :
+    <<PRESERVED: forall b_src delta (NOW: f_new b_src = Some (b_tgt, delta)),
+      <<OLD: f_old b_src = Some (b_tgt, delta)>> >>
+.
+Proof.
+  inv FROZEN.
+  ii.
+  destruct (f_old b_src) eqn:T; ss.
+  - destruct p; ss.
+    exploit INJECT; eauto; []; i; des.
+    clarify.
+  - exfalso.
+    exploit NEW_IMPLIES_OUTSIDE; eauto; []; i; des.
+    xomega.
+Qed.
+
+Lemma frozen_shortened
+      f_old f_new
+      bd_src0 bd_tgt0
+      (FROZEN: frozen f_old f_new bd_src0 bd_tgt0)
+      bd_src1 bd_tgt1
+      (SHORT_SRC: (bd_src1 <= bd_src0)%positive)
+      (SHORT_TGT: (bd_tgt1 <= bd_tgt0)%positive)
+  :
+    <<FROZEN: frozen f_old f_new bd_src1 bd_tgt1>>
+.
+Proof.
+  inv FROZEN.
+  econs; eauto.
+  ii. des.
+  hexploit NEW_IMPLIES_OUTSIDE; eauto; []; i; des. clear NEW_IMPLIES_OUTSIDE.
+  split; ss.
+  - red. etransitivity; eauto.
+  - red. etransitivity; eauto.
+Qed.
+
+Lemma frozen_refl
+      f
+      bound_src bound_tgt
+  :
+    <<FROZEN: frozen f f bound_src bound_tgt>>
+.
+Proof.
+  econs; eauto. i; des. clarify.
+Qed.
+
+Lemma loc_unmapped_frozen
+      F F'
+      fbound_src fbound_tgt
+      (FROZEN : frozen F F' fbound_src fbound_tgt)
+      b ofs
+      (BOUND: Plt b fbound_src)
+      (UNMAPPED: loc_unmapped F b ofs)
+  :
+    loc_unmapped F' b ofs
+.
+Proof.
+  unfold loc_unmapped in *.
+  destruct (F' b) eqn:T; ss.
+  destruct p; ss.
+  inv FROZEN.
+  exploit NEW_IMPLIES_OUTSIDE; eauto.
+  i; des. xomega.
+Qed.
+
+Lemma loc_out_of_reach_frozen
+      F F'
+      fbound_src fbound_tgt
+      (INCR: inject_incr F F')
+      (FROZEN : frozen F F' fbound_src fbound_tgt)
+      b ofs
+      (BOUND: Plt b fbound_tgt)
+      m0 m1
+      (UNMAPPED: loc_out_of_reach F m0 b ofs)
+      (UNCHANGED: forall k p b0 delta (MAPPED: F b0 = Some (b, delta)),
+          Mem.perm m0 b0 (ofs - delta) k p <-> Mem.perm m1 b0 (ofs - delta) k p)
+  :
+    loc_out_of_reach F' m1 b ofs
+.
+Proof.
+  unfold loc_out_of_reach in *.
+  i.
+  exploit frozen_preserves_tgt; eauto.
+  i. des.
+  hexploit UNMAPPED; eauto. i.
+  ii.
+  contradict H1.
+  eapply UNCHANGED; eauto.
+Qed.
+
+
+Section MEMINJ.
+
+Local Existing Instance Val.mi_normal.
+(* Variable gbound_src gbound_tgt: block. *)
+
+Record t' := mk {
+  inj: meminj;
+  m_src: mem;
+  m_tgt: mem;
+  inj_parent: meminj;
+  m_src_parent: mem;
+  m_tgt_parent: mem;
+}.
+
+Definition valid_blocks (m: mem): block -> Z -> Prop := fun b _ => m.(Mem.valid_block) b.
+Hint Unfold valid_blocks.
+
+Definition src_private (sm: t'): block -> Z -> Prop :=
+  loc_unmapped sm.(inj) /2\ sm.(m_src).(valid_blocks)
+.
+
+Definition tgt_private (sm: t'): block -> Z -> Prop :=
+  loc_out_of_reach sm.(inj) sm.(m_src) /2\ sm.(m_tgt).(valid_blocks)
+.
+
+Definition src_private_parent (sm: t'): block -> Z -> Prop :=
+  loc_unmapped sm.(inj_parent) /2\ sm.(m_src_parent).(valid_blocks)
+.
+
+Definition tgt_private_parent (sm: t'): block -> Z -> Prop :=
+  loc_out_of_reach sm.(inj_parent) sm.(m_src_parent) /2\ sm.(m_tgt_parent).(valid_blocks)
+.
+Hint Unfold src_private tgt_private src_private_parent tgt_private_parent.
+
+Inductive wf' (rel: t'): Prop :=
+| wf_intro
+    (PUBLIC: Mem.inject rel.(inj) rel.(m_src) rel.(m_tgt))
+    (SRCPBOUND: (rel.(m_src_parent).(Mem.nextblock) <= rel.(m_src).(Mem.nextblock))%positive)
+    (TGTPBOUND: (rel.(m_tgt_parent).(Mem.nextblock) <= rel.(m_tgt).(Mem.nextblock))%positive)
+    (PUBLICPARENT: Mem.inject rel.(inj_parent) rel.(m_src_parent) rel.(m_tgt_parent))
+.
+
+Lemma wf_corollary
+      sm0
+      (WF: wf' sm0)
+  :
+    sm0.(src_private_parent) <2= sm0.(src_private)
+.
+Proof.
+  u.
+  ii; ss. des; ss. inv WF.
+  unfold loc_unmapped in *.
+  esplits; eauto.
+  -
+Qed.
+
+Inductive le' (mrel0 mrel1: t'): Prop :=
+| le_intro
+    (INCR: inject_incr mrel0.(inj) mrel1.(inj))
+    (SRCUNCHANGED: Mem.unchanged_on mrel0.(src_private_parent) mrel0.(m_src) mrel1.(m_src))
+    (TGTUNCHANGED: Mem.unchanged_on mrel0.(tgt_private_parent) mrel0.(m_tgt) mrel1.(m_tgt))
+    (SRCPARENTEQ: mrel0.(m_src_parent) = mrel1.(m_src_parent))
+    (TGTPARENTEQ: mrel0.(m_tgt_parent) = mrel1.(m_tgt_parent))
+    (INJPARENTEQ: mrel0.(inj_parent) = mrel1.(inj_parent))
+    (FROZEN: frozen mrel0.(inj) mrel1.(inj) (mrel0.(m_src_parent).(Mem.nextblock))
+                                            (mrel0.(m_tgt_parent).(Mem.nextblock)))
+    (SRCBOUND: (mrel0.(m_src).(Mem.nextblock) <= mrel1.(m_src).(Mem.nextblock))%positive)
+    (TGTBOUND: (mrel0.(m_tgt).(Mem.nextblock) <= mrel1.(m_tgt).(Mem.nextblock))%positive)
+.
+
+Definition lift' (mrel0: t'): t' :=
+  (mk mrel0.(inj) mrel0.(m_src) mrel0.(m_tgt)
+      mrel0.(inj) mrel0.(m_src) mrel0.(m_tgt))
+.
+
+Definition unlift' (mrel0 mrel1: t'): t' :=
+  (mk mrel1.(inj) mrel1.(m_src) mrel1.(m_tgt)
+      mrel0.(inj_parent) mrel0.(m_src_parent) mrel0.(m_tgt_parent))
+.
+
+(* TODO: Let's have this as policy. (giving explicit name) *)
+(* TODO: apply this policy for identity/extension *)
+
+(* "Global" is needed as it is inside section *)
+Global Program Instance SimMemInj : SimMem.class :=
+{
+  t := t';
+  src_mem := m_src;
+  tgt_mem := m_tgt;
+  wf := wf';
+  le := le';
+  lift := lift';
+  unlift := unlift';
+  sim_val := fun (mrel: t') => Val.inject mrel.(inj);
+}.
+Next Obligation.
+  econs.
+  - i. econs; eauto; try reflexivity; try apply Mem.unchanged_on_refl; eauto.
+    { eapply frozen_refl; eauto. }
+  - ii. inv H; inv H0.
+    econs; eauto with mem congruence.
+    + eapply inject_incr_trans; eauto.
+    + eapply Mem.unchanged_on_trans; eauto with congruence.
+      unfold src_private_parent in *.
+      eapply Mem.unchanged_on_implies; eauto with mem congruence.
+    + eapply Mem.unchanged_on_trans; eauto with congruence.
+      unfold tgt_private_parent in *.
+      eapply Mem.unchanged_on_implies; eauto with mem congruence.
+    + econs; eauto.
+      ii; des.
+      destruct (inj y b_src) eqn:T.
+      * destruct p.
+        exploit INCR0; eauto. i; clarify.
+        inv FROZEN.
+        hexploit NEW_IMPLIES_OUTSIDE; eauto.
+      * inv FROZEN0.
+        hexploit NEW_IMPLIES_OUTSIDE; eauto; []; i; des.
+        split; ss.
+        rewrite SRCPARENTEQ. ss.
+        rewrite TGTPARENTEQ. ss.
+    + etransitivity; eauto.
+    + etransitivity; eauto.
+Qed.
+Next Obligation.
+  rename H into VALID.
+  inv VALID. econs; ss; eauto; ii; des; ss; eauto.
+  - eapply Pos.compare_gt_iff in H. xomega.
+  - eapply Pos.compare_gt_iff in H. xomega.
+  (* - econs; eauto. *)
+  (*   ii; des. clarify. *)
+  (* - eapply Mem.unchanged_on_refl. *)
+  (* - eapply Mem.unchanged_on_refl. *)
+Qed.
+Next Obligation.
+  inv H; ss.
+  econs; ss; eauto; ii; des; ss.
+  - eapply Mem.unchanged_on_implies; eauto.
+    unfold src_private_parent in *. unfold loc_unmapped in *.
+    i; des. esplits; eauto. cbn in *.
+    inv H0. inv FROZEN.
+    destruct (inj mrel0 b) eqn:T; ss. destruct p; ss. exfalso.
+    exploit NEW_IMPLIES_OUTSIDE; eauto. i; des.
+    u in *. unfold Mem.valid_block in *. xomega.
+  - eapply Mem.unchanged_on_implies; eauto.
+    unfold tgt_private_parent in *. ii; des. esplits; eauto.
+    inv H0. ss.
+    eapply loc_out_of_reach_frozen; eauto.
+    ii. eapply SRCUNCHANGED0; eauto.
+    { hnf. u. esplits; eauto.
+    unfold loc_out_of_reach in *.
+    ii; des. esplits; eauto. ii. cbn in *.
+    inv H0. inv FROZEN.
+    destruct (inj_parent mrel0 b0) eqn:T; cycle 1; ss.
+    {
+    { destruct p; ss. exploit INCR0; eauto. i; des. clarify. exploit H; eauto. i; des. eauto with mem.
+                                                eauto. exfalso.
+    exploit NEW_IMPLIES_OUTSIDE; eauto. i; des.
+    u in *. unfold Mem.valid_block in *. xomega.
+  - eapply Mem.unchanged_on_implies; eauto.
+    i. esplits; eauto. eapply H0; eauto.
+  - inv H0. ss.
+    eapply frozen_shortened; eauto.
+Qed.
+Next Obligation.
+  inv H. inv H0. inv H1.
+  econs; ss; eauto. (* eauto did well here *)
+  - etransitivity; eauto.
+    inv FROZEN. unfold valid_blocks in *.
+    ii. des; ss. esplits; eauto.
+    + hnf. destruct (inj mrel1 x0) eqn:T; ss. destruct p; ss.
+      exploit NEW_IMPLIES_OUTSIDE.
+      { esplits; eauto. }
+      i. des. inv PUBLIC. ss.
+  - etransitivity; eauto.
+Qed.
+Next Obligation.
+  ii. inv MLE. eapply val_inject_incr; eauto.
+Qed.
+
+End MEMINJ.
+
+
+
+
+
+
+
+
+
+
+
+
+
+Inductive sim_skenv (skenv0 skenv1: SkEnv.t): Prop :=
+| sim_skenv_intro
+    (NEXT: skenv0.(Genv.genv_next) = skenv1.(Genv.genv_next))
+    (SYMB: all1 (skenv0.(Genv.find_symbol) =1= skenv1.(Genv.find_symbol)))
+    (DEFS: all1 (skenv0.(Genv.find_def) =1= skenv1.(Genv.find_def)))
+    (PUBS: skenv0.(Genv.genv_public) = skenv1.(Genv.genv_public))
+.
+
+Inductive skenv_inject (skenv: SkEnv.t) (j: meminj): Prop :=
+| sken_inject_intro
+    (DOMAIN: forall b, Plt b skenv.(Genv.genv_next) -> j b = Some(b, 0))
+    (IMAGE: forall b1 b2 delta, j b1 = Some(b2, delta) -> Plt b2 skenv.(Genv.genv_next) -> b1 = b2)
+.
+
+Inductive sim_skenv_inj (sm: SimMem.t) (__noname__: unit) (skenv_src skenv_tgt: SkEnv.t): Prop :=
+| sim_skenv_inj_intro
+    (INJECT: skenv_inject skenv_src sm.(inj))
+    (BOUNDSRC: Ple skenv_src.(Genv.genv_next) sm.(m_src_parent).(Mem.nextblock))
+    (BOUNDTGT: Ple skenv_src.(Genv.genv_next) sm.(m_tgt_parent).(Mem.nextblock))
+    (SIMSKENV: sim_skenv skenv_src skenv_tgt)
+.
+
+Inductive sim_sk (u: unit) (sk_src sk_tgt: Sk.t): Prop :=
+| sim_sk_intro
+    (SIM: match_program (fun _ => sim_fun) eq sk_src sk_tgt)
+.
+
+Global Program Instance SimSymbId: SimSymb.class SimMemInj := {
+  t := unit;
+  le := top4;
+  sim_sk := sim_sk;
+  sim_skenv := sim_skenv_inj;
+}
+.
+Next Obligation.
+  inv SIMSK. inv SIMSK0.
+  SearchAbout TransfLink.
+  admit "this should hold".
+Qed.
+Next Obligation.
+  u in *. inv SIMSK.
+  Print Genv.init_mem_transf.
+  Print Genv.init_mem_transf_partial.
+  About Genv.init_mem_match.
+  exploit (Genv.init_mem_match SIM); eauto. i. clarify.
+  esplits; eauto.
+  - instantiate (1:= mk (Mem.flat_inj m_src.(Mem.nextblock))
+                                  bot2 bot2 bot2 bot2 m_src m_src m_src m_src).
+    econs; ss; eauto.
+    + econs; eauto; ii; ss.
+      * unfold Mem.flat_inj in *. erewrite ! Genv.init_mem_genv_next in *; eauto. des_ifs.
+      * unfold Mem.flat_inj in *. erewrite ! Genv.init_mem_genv_next in *; eauto. des_ifs.
+    + ss. erewrite ! Genv.init_mem_genv_next; eauto. reflexivity.
+    + ss. erewrite ! Genv.init_mem_genv_next; eauto. reflexivity.
+    + econs; eauto.
+      * erewrite ! Genv.init_mem_genv_next; eauto.
+      * i. symmetry. apply (Genv.find_symbol_match SIM).
+      * ii. hexploit (Genv.find_def_match_2 SIM x0); eauto. intro REL.
+        inv REL; ss. inv H2; ss.
+        { admit "remove sig then this will hold // or just now this will hold if we don't drop sig on opt". }
+        inv H3; ss.
+      * inv SIM; des; ss. rewrite ! Genv.globalenv_public. ss.
+  - ss.
+  - ss.
+  - econs; ss; try xomega; ii; des; ss; eauto.
+    eapply Genv.initmem_inject; eauto.
+Unshelve.
+Qed.
+Next Obligation.
+  assert(BOUNDSRC: Ple (Genv.genv_next skenv_src) (Mem.nextblock (m_src_parent sm1))).
+  { inv MLE. rewrite <- SRCPARENTEQ. eapply SIMSKENV. }
+  assert(BOUNDTGT: Ple (Genv.genv_next skenv_src) (Mem.nextblock (m_tgt_parent sm1))).
+  { inv MLE. rewrite <- TGTPARENTEQ. eapply SIMSKENV. }
+  inv SIMSKENV. inv INJECT.
+  econs; eauto.
+  econs; eauto.
+  - ii. exploit DOMAIN; eauto. i. eapply MLE; eauto.
+  - ii. inv MLE.
+    eapply IMAGE; eauto.
+    erewrite frozen_preserves_tgt; eauto.
+    eapply Plt_Ple_trans; eauto.
+Qed.
+Next Obligation.
+  inv MWF. inv SIMSKENV.
+  econs; eauto.
+  - etransitivity; try apply SRCPBOUND. ss.
+  - etransitivity; try apply TGTPBOUND. ss.
+Qed.
+Next Obligation.
+  inv LESRC.
+  inv LETGT.
+  inv SIMSKENV. inv SIMSKENV0.
+  inv SIMSK. unfold match_program in *.
+  assert(DEFSEQ: sk_src.(defs) = sk_tgt.(defs)).
+  { apply Axioms.functional_extensionality. intro id.
+    hexploit (@match_program_defmap _ _ _ _ _ _ _ _ _ _ _ SIM).
+    instantiate (1:= id).
+    i.
+    inv H; ss.
+    - unfold defs.
+      admit "this is weak. add list_norept or prove my own theorem with induction.".
+    - admit "this will hold".
+  }
+  econs; eauto.
+  { inv INJECT.
+    econs; ii; eauto.
+    - eapply DOMAIN; eauto. rewrite NEXT. ss.
+    - eapply IMAGE; eauto. rewrite NEXT. ss.
+  }
+  { rewrite <- NEXT. ss. }
+  { rewrite <- NEXT. ss. }
+  econs; eauto.
+  - eq_closure_tac.
+  - intro id.
+    destruct (Classical_Prop.classic (sk_src.(defs) id)); cycle 1.
+    + exploit SYMBDROP; eauto. i; des.
+      exploit SYMBDROP0; eauto. { rewrite <- DEFSEQ. eauto. } i; des.
+      rewrite H0. rewrite H1. ss.
+    + exploit SYMBKEEP; eauto. i; des.
+      exploit SYMBKEEP0; eauto. { rewrite <- DEFSEQ. eauto. } i; des.
+      rewrite H0. rewrite H1. ss.
+  - intro blk.
+    destruct (Genv.invert_symbol skenv_link_src blk) eqn:T0; cycle 1.
+    + rewrite DEFORPHAN; ss.
+      destruct (Genv.invert_symbol skenv_link_tgt blk) eqn:T1; cycle 1.
+      * rewrite DEFORPHAN0; ss.
+      * repeat all_once_fast ltac:(fun H => try apply Genv.invert_find_symbol in H; des).
+        rewrite <- SYMB in *.
+        repeat all_once_fast ltac:(fun H => try apply Genv.find_invert_symbol in H; des).
+        clarify.
+    + destruct (Genv.invert_symbol skenv_link_tgt blk) eqn:T1; cycle 1.
+      * repeat all_once_fast ltac:(fun H => try apply Genv.invert_find_symbol in H; des).
+        rewrite SYMB in *.
+        repeat all_once_fast ltac:(fun H => try apply Genv.find_invert_symbol in H; des).
+        clarify.
+      * repeat all_once_fast ltac:(fun H => try apply Genv.invert_find_symbol in H; des).
+        assert(i = i0).
+        { eapply Genv.genv_vars_inj; eauto. unfold Genv.find_symbol in *. rewrite SYMB. ss. }
+        clarify.
+        repeat all_once_fast ltac:(fun H => try apply Genv.find_invert_symbol in H; des).
+        destruct (classic (defs sk_src i0)).
+        { erewrite DEFKEEP; eauto. erewrite DEFKEEP0; eauto. rewrite <- DEFSEQ; ss. }
+        { erewrite DEFDROP; eauto. erewrite DEFDROP0; eauto. rewrite <- DEFSEQ; ss. }
+  - rewrite PUBLIC. rewrite PUBLIC0. ss.
+Qed.
+Next Obligation.
+  inv SIMSKENV. inv SIMSKENV0. inv INJECT.
+  econs; eauto.
+  - ii. ss.
+    assert(fptr_src = fptr_tgt).
+    { inv SIMFPTR; ss. des_ifs. rewrite Ptrofs.add_zero_l.
+      unfold Genv.find_funct, Genv.find_funct_ptr in *. des_ifs_safe.
+      exploit DOMAIN; eauto. { eapply Genv.genv_defs_range; eauto. } i; clarify. }
+    clarify. unfold Genv.find_funct, Genv.find_funct_ptr in *. des_ifs_safe.
+    erewrite <- DEFS; eauto. des_ifs. esplits; eauto.
+    admit "just use eq".
+  - ii.
+    assert(fptr_src = fptr_tgt).
+    { inv SIMFPTR; ss. des_ifs.
+      unfold Genv.find_funct, Genv.find_funct_ptr in *. des_ifs_safe.
+      exploit IMAGE; eauto. { rewrite NEXT. eapply Genv.genv_defs_range; eauto. } i; clarify.
+      exploit DOMAIN; eauto. { rewrite <- DEFS in *. eapply Genv.genv_defs_range; eauto. } i; clarify.
+      rewrite e. rewrite Ptrofs.add_zero in *. clarify.
+    }
+    clarify. unfold Genv.find_funct, Genv.find_funct_ptr in *. des_ifs_safe.
+    erewrite DEFS; eauto. des_ifs. esplits; eauto.
+    admit "just use eq".
+Qed.
+
